\section{Листок}

\begin{exercise}
Доказать, что 	$\displaystyle\int_{0}^{\infty} \frac{t^{2 n-1}}{e^{2 \pi t}-1} d t=\frac{1}{4 n}\left| B_{2 n}\right| $ , где $B_{n}$ - числа Бернулли.
$$ \displaystyle \frac{x}{e^{x}-1}=\sum_{n=0}^{\infty} \frac{B_{n} x^{n}}{n !}$$

\end{exercise}
\begin{solution}
	$$
	\int_{0}^{\infty} \frac{t^{2 n-1}}{e^{2 n t}-1} d t=\int_{0}^{\infty} d t \frac{t^{2 n-1}}{e^{2 \pi t}}\left(1-e^{-2 \pi t}\right)^{-1} = \int_{0}^{\infty}  d t \hspace{2pt} t^{2 n-1} \sum_{k=0}^{\infty} e^{-2 \pi k t}=\sum_{k = 0}^{\infty} \int_{0}^{\infty} d t \hspace{2pt} \frac{t^{2 n-1}}{e^{2 \pi t}} e^{-2 \pi k t}
	$$
	
	$$
	\sum_{k=0}^{\infty} \int_{0}^{\infty} d t \hspace{2pt} t^{2 n-1} e^{-2 \pi(k+1) t} = \left|
	\begin{array}{l}{x=2 \pi(k+1) t} \\ {d x=2 \pi(k+1) d t}\end{array} \right|=\sum_{k=0}^{\infty} \int_{0}^{\infty} \frac{d x}{2 \pi(k+1)} \frac{x^{2 n-1} e^{-x}}{(2 \pi(k+1))^{2 n-1}} d x
	$$
	
	$$
	\sum_{k=0}^{\infty} \frac{1}{(2 \pi(k+1))^{2 n}} \int_{0}^{\infty} d x \hspace{2pt} x^{2 n-1} e^{-x} = \frac{1}{(2 \pi)^{2n}}\sum_{k=1}^{\infty} \frac{1}{k^{2 n}} \hspace{2pt} \Gamma(2 n) = \frac{1}{(2 \pi)^{2 n}} \zeta(2 n) \cdot \Gamma(2 n) = 
	$$
	
	$$
	\left|\Gamma(2n)=(2 n-1) ! \qquad \zeta(2 n)=\frac{(-1)^{n+1} B_{2 n}(2 \pi)^{2 n}}{2(2 n) !} \right|
	$$
	
	$$
	= (-1)^{n+1} \frac{B_{2 n}}{4 n}
	$$
	
\end{solution}