\section{Лекция 2}

\begin{problem}
	content...
\end{problem}

\begin{problem}
	content...
\end{problem}




\begin{problem}
	$T(a, b)=\nabla_{a} b-\nabla_{b} a-[a, b] \quad(\forall a, b \in C(T M)) \quad \Leftrightarrow \quad T_{\mu \nu}^{\lambda}=\Gamma_{\nu \mu}^{\lambda}-\Gamma_{\mu \nu}^{\lambda}$
\end{problem}	

\begin{solution}
	$$\nabla_{a} b-\nabla_{b} a-[a, b]=0$$
	$$
	a^{\mu} \nabla_{\mu} b-b^{\mu} \nabla_{\mu} a-a b+b a
	$$
	$$
	a^{\mu}\left(\partial_{\mu} b^{\lambda}\right) \partial_{\lambda} 
	- b^{\mu}\left(\partial_{\mu} a^{\lambda}\right) \partial_{\lambda}
	+ 
	a^{\mu} \Gamma_{\nu \mu}^{\lambda} b^{\nu} \partial_{\lambda}
	-	b^{\mu} \Gamma_{\nu \mu}^{\lambda} a^{\nu} \partial_{\lambda}
	+a^{\mu}\partial_{\mu} b^{k}\partial_{k}-
	b^{\mu}\partial_{\mu} a^{k}\partial_{k}
	$$
	$$
	a^{\mu} \Gamma_{\nu \mu}^{\lambda} b^{\nu} \partial_{\lambda}=b^{\mu} \Gamma_{\nu \mu}^{\lambda} a^{\nu} \partial_{\lambda}
	$$
	$$
	a^{\mu} b^{\nu} \Gamma_{\nu \mu}^{\lambda}=a^{\mu} b^{\nu} \Gamma_{\mu \nu}^{\lambda} \quad \forall a^{\mu}, b^{\nu}  \in	C(T M)
	$$
	$$
	\boxed{\Gamma_{\nu \mu}^{\lambda}-\Gamma_{\mu \nu}^{\lambda}}
	$$
	
	
	
\end{solution}

